current status: adequacy theorem / pi-injectivity stated. many admits.

theories/examples/finelt/raw_validity2.v
@@ -9,6 +9,10 @@ Set Implicit Arguments.
 Unset Strict Implicit.
 Unset Printing Implicit Defensive.
 
+Require Import smpl.Smpl.
+Require Import utils.all.
+
+
 
 Require Import syntax.syntax.
 Require Import syntax.typing.
@@ -50,6 +54,21 @@ Proof.
   - inversion H5.
   - inversion H2.
   - rewrite (@IHM1 M3 M5) ; eauto.
+Qed.
+
+Lemma HeadRed_tpi_det (n:nat) (M : Tm n) A1 B1 A2 B2 : 
+  HeadRed M (Core.tpi A1 B1) -> HeadRed M (Core.tpi A2 B2) ->
+  A1 = A2 /\ B1 = B2.
+Proof.
+  move=> h1. move:A2 B2.
+  dependent induction h1.
+  all: move=> A2 B2 h2. 
+  - inversion h2; subst. done. inversion H.
+  - inversion h2; subst. inversion H.
+    specialize (IHh1 _ _ ltac:(reflexivity) A2 B2).
+    have EQ: e2 = e3. eapply HeadRed1_det; eauto.
+    subst.
+    eauto.
 Qed.
 
 Require Import findom.
@@ -103,17 +122,24 @@ Lemma wt_succ_inv u:
 move=>h. inversion h. done. Defined.
 
 
-(* Logical relation, defined by induction on (semantic type) a.
-   We only need it for closed terms, so dropping the context and 
-   specializing M's scope to 0.
+(* Logical relation, defined by recursion on the wt judgement for 
+   semantic elements. i.e. on the derivation of `wt u a`.
 
-   As a is "more defined" this set becomes smaller. When we don't 
-   know anything, i.e. a is bot, then we have the total set.
+   We only need the relation for closed terms, so compared to the 
+   Agda version, this code drops the context and specializes M's 
+   scope to 0.
 
-   NOT TRUE: If Val M A (h: wt u a) holds 
-             then we know that null |- M : A
- *)
+   This is a coinductive definition. As u is "more defined" the 
+   set of syntactic terms in the relation becomes smaller. 
+   To begin, when u is bot, it is the total set.
 
+*)
+
+
+(* This module defines various helper operations on the logical 
+   relation. Each of these operations is parameterized by the 
+   two main fixpoints (Val and EqVal). 
+*)
 Module Rec.
 Section Helpers.
 
@@ -210,11 +236,11 @@ Fixpoint
              (* both reduce to pi types *)
              exists A B, HeadRed M (Core.tpi A B) 
              /\ exists A' B', HeadRed N (Core.tpi A' B') 
-             (* that are well-typed *)
+             (* ... that are well-typed *)
              /\ conv ctx_empty A A' (Core.tuniv i)
              /\ conv (ctx_empty ++ A) B B' (Core.tuniv i)
              /\ valid (tpi b f)
-             (* domain is in the relation *)
+             (* ... and the domain is in the relation *)
              /\ EqVal A A' (Core.tuniv i) (wt_tpi_dom h)
         /\ (* PiEdgeEqTy A B B' h *)
              (forall u v (IN : In (u,v) f) (P : Tm 0), 
@@ -250,7 +276,6 @@ Fixpoint Val
             end) h
 
       | tnat => fun h =>
-          HeadRed A (Core.tnat) /\
           (match u return wt _ tnat -> Prop with 
                | zero => fun h => 
                  HeadRed M (Core.zero)
@@ -280,7 +305,7 @@ with EqVal
            | bot => fun h => True 
            | abs g => fun (h : wt (abs g) (tpi b f)) => 
                      
-             (* this is not available *)
+             (* this is not available, b/c wt doesn't check domain type *)
              (* ValTy Val EqVal A (wt_abs_dom h) *)
                Rec.ValPi Val M A h
              /\ Rec.ValPi Val N A h
@@ -290,7 +315,6 @@ with EqVal
             end) h
 
       | tnat => fun h =>
-          HeadRed A (Core.tnat) /\
           (match u return wt _ tnat -> Prop with 
                | zero => fun h => 
                  HeadRed M Core.zero
@@ -325,6 +349,25 @@ Proof.
 Abort.
 
 
+(* ============================================================
+   Val2-Bot, EqVal2-Bot: at u = bot, both relations are True. 
+   ============================================================ *)
+
+Lemma Val_Bot M A a (h : wt bot a) : Val M A h.
+Proof. dependent destruction h.
+       destruct a eqn:EQa; try done.
+Qed.
+
+Lemma EqVal_Bot M N A a (h : wt bot a) : EqVal M N A h.
+Proof. 
+dependent destruction h.
+       destruct a eqn:EQa; try done.
+Qed.
+
+
+(* ============================================================
+   Val <-> ValTy  and  EqVal <-> EqValTy
+   ============================================================ *)
 
 Lemma EqValTy_EqVal A B a i (h : wt a (tuniv i)):
   EqValTy A B h ->
@@ -345,6 +388,27 @@ Proof.
   all: eauto.
 Qed.
 
+Lemma ValTy_Val A a i (h : wt a (tuniv i)):
+  ValTy A h ->
+  Val A (Core.tuniv i) h.
+Proof.
+  dependent destruction h; try done.
+Qed.
+
+Lemma Val_ValTy A a i (h : wt a (tuniv i)):
+  Val A (Core.tuniv i) h ->
+  ValTy A h.
+Proof.
+  dependent destruction h; try done.
+Qed.
+
+
+(* ============================================================
+   Diagonal embedding
+   Val <-> EqVal  and  ValTy → EqValTy
+   ============================================================ *)
+
+
 Fixpoint Val_EqVal M A u a (h : wt u a) {struct h} : 
   Val M A h -> EqVal M M A h.
 Proof.
@@ -352,8 +416,7 @@ Proof.
   all: cbn.
   all: eauto.
   - destruct a; try done.
-  - move=> [hA [M1 [h1 V1]]].
-    split; auto.
+  - move=> [M1 [h1 V1]].
     exists M1. split; auto.
     exists M1. split; auto.
   - move=>h1.  
@@ -382,6 +445,23 @@ Proof.
 Qed.
     
 
+(* ValTy2-to-EqValTy2 *)
+Lemma ValTy_EqValTy M u i (h : wt u (tuniv i)) :
+  ValTy M h -> EqValTy M M h.
+Proof.
+  intros VT.
+  eapply EqVal_EqValTy.
+  eapply Val_EqVal.
+  eapply ValTy_Val.
+  auto.
+Qed.
+
+
+(* ============================================================
+   Level 1 — projecting first and second parts of EqVal
+   EqVal_Val1, EqVal_Val2
+   ============================================================ *)
+
 
 Fixpoint EqVal_Val1 M N A u a (h : wt u a) {struct h} : 
   EqVal M N A h -> Val M A h.
@@ -391,8 +471,7 @@ Proof.
   all: eauto.
   (* 2 nontrivial goals *)
   - destruct a; try done.
-  - move=> [hA [M1 [h1 [N1 [h2 V1]]]]].
-    split; auto.
+  - move=> [M1 [h1 [N1 [h2 V1]]]].
     exists M1. split; auto.
     eauto.
 Qed.
@@ -406,409 +485,820 @@ Proof.
   all: eauto.
   (* 2 nontrivial goals *)
   - destruct a; try done.
-  - move=> [hA [M1 [h1 [N1 [h2 V1]]]]].
-    split; auto.
+  - move=> [M1 [h1 [N1 [h2 V1]]]].
     exists N1. split; auto.
     eauto.
 Qed.
 
-(* 
+(* ============================================================
+   Level 1a — 
+   Head reduction/expansion
+   ============================================================ *)
 
-  upVal2 : {n : Nat} (G : Ctx n) (M T : Expr n) (u a0 a1 : FinEl) ->
-    LeCode a0 a1 -> FinMem u a0 -> FinMem u a1 ->
-    Coherent a0 -> Coherent a1 ->
-    Val2 G M T u a0 -> ValTy2 G T a1 ->
-    Val2 G M T u a1
-  upEqVal2 : {n : Nat} (G : Ctx n) (M N T : Expr n) (u a0 a1 : FinEl) ->
-    LeCode a0 a1 -> FinMem u a0 -> FinMem u a1 ->
-    Coherent a0 -> Coherent a1 ->
-    EqVal2 G M N T u a0 -> ValTy2 G T a1 ->
-    EqVal2 G M N T u a1
 
+(* ValTy2-headred-expand *)
+Lemma ValTy_headred_expand M M' u i (h : wt u (tuniv i)) :
+  HeadRed M' M -> ValTy M h -> ValTy M' h.
+Proof. Admitted.
+
+(* ValTy2-headred-contract *)
+Lemma ValTy_headred_contract M M' u i (h : wt u (tuniv i)) :
+  HeadRed M M' -> ValTy M h -> ValTy M' h.
+Proof. Admitted.
+
+
+(* ============================================================
+   down/up
+   ============================================================ *)
+
+(* Annoyingly, struct on first derivation is not enough. Need 
+   to do struct on *both* wt derivations simultaneously to 
+   show the termination of this proof. 
+
+   For now, admitting the termination check.
 *)
 
-Fixpoint upVal M T u a0 a1 i 
-  (h0 : wt u a0) (h1 : wt u a1) (ha1 : wt a1 (tuniv i)) {struct h0}:
-  le a0 a1 -> Val M T h0 -> ValTy T ha1 -> Val M T h1
-with upEqVal M N T u a0 a1 i 
-  (h0 : wt u a0) (h1 : wt u a1) (ha1 : wt a1 (tuniv i)) {struct h0}:
-  le a0 a1 -> EqVal M N T h0 -> ValTy T ha1 -> EqVal M N T h1
-.
-Proof.
-  dependent destruction h0.
-  + dependent destruction h1.
-    move=> LE VB VT.
-    cbn in VB. cbn.
-    destruct a; destruct a0; cbn; auto. 
-    all: dependent destruction ha1.
-    all: cbn in LE; try done.
-    all: cbn in VT.
-    admit.
-  + 
-Admitted.
-
-Fixpoint downVal M T u a0 a1 
+Fixpoint upVal M T u a0 a1  
+  (h0 : wt u a0) (h1 : wt u a1) {struct h0}:
+  le a0 a1 -> Val M T h0 -> Val M T h1
+with upEqVal M N T u a0 a1  
+  (h0 : wt u a0) (h1 : wt u a1) {struct h0}:
+  le a0 a1 -> EqVal M N T h0 -> EqVal M N T h1
+with downVal M T u a0 a1 
   (h0 : wt u a0) (h1: wt u a1) {struct h1} : 
   le a0 a1 -> Val M T h1 -> Val M T h0
 with downEqVal M N T u a0 a1 
   (h0 : wt u a0) (h1: wt u a1) {struct h1} : 
   le a0 a1 -> EqVal M N T h1 -> EqVal M N T h0.
 Proof.
-  - dependent destruction h1.
-    all: dependent destruction h0.
+  - (* upVal *)
+    dependent destruction h1;
+    dependent destruction h0.
+    all: try solve [cbn; eauto].
+    + (* bot *)
+      destruct a; destruct a0; cbn; auto.
+    + (* tnat *)
+      move=> _ [M1 [RM1 VM1]].
+      exists M1. split. auto.
+      eapply upVal with (a1 := tnat); eauto. 
+      done.
+    + (* tuniv *)
+      move=> LE VT.
+      cbn in LE. 
+      apply Nat.eqb_eq in LE. subst j0.
+      have EQ: (wt_tpi w w0 h0 i = wt_tpi w1 w2 h1 i0) by ext.
+      (* proof irrelevance for wt? this case doesn't use recursion *)
+      rewrite <- EQ.
+      eapply VT.
+    + (* tpi *)
+      rewrite le_tpi. cbn. unfold ValPi, PiAppVal.
+      move=> /andP. move=> [LEa LEg] [A [B [R1 h1]]]. 
+
+      move: (andb_prop _ _ i0) => [Va Vg]. 
+      fold valid in Va.
+      fold valid in Vg. fold (valid_fun g) in Vg.
+      move: (andb_prop _ _ i2) => [Va0 Vg0]. 
+      fold valid in Va0. 
+      fold valid in Vg0. fold (valid_fun g0) in Vg0.
+
+      exists A, B. split; auto.
+      move=> u v INf P t0 APP0 TA VP.
+      specialize (h1 u v INf P).
+      have Vu : valid u. eauto with valid.
+      destruct (valid_app_exists Vg Vu) as [t [APP Vt]].
+      move: (le_fun_mono Vg Vg0 LEg Vu APP APP0) => LEt.
+
+      cbn.
+      eapply upVal. 
+      Unshelve. eapply LEt. 2: { eapply (w0 _ _ _ INf APP). } 
+      eapply h1. eapply TA.
+      cbn.
+      eapply downVal. eapply LEa. 
+      Unshelve. cbn in VP. 2: { eapply (w1 _ _ _ INf APP0). }  
+      eapply VP.
+      
+  - (* upEqVal *)
+    dependent destruction h1;
+    dependent destruction h0.
+    all: try solve [cbn; eauto].
+    + (* bot *)
+      destruct a; destruct a0; cbn; auto.
+    + (* tnat *)
+      move=> _ [M1 [RM1 [N1 [RN1 VM1]]]].
+      exists M1. split. auto.
+      exists N1. split. auto.
+      eapply upEqVal with (a1 := tnat); eauto. 
+      done.
+    + (* tuniv *)
+      move=> LE VT.
+      cbn in LE. 
+      apply Nat.eqb_eq in LE. subst j0.
+      have EQ: (wt_tpi w w0 h0 i = wt_tpi w1 w2 h1 i0) by ext.
+      (* proof irrelevance for wt? this case doesn't use recursion *)
+      rewrite <- EQ.
+      eapply VT.
+    + (* tpi *)
+      rewrite le_tpi. cbn. unfold ValPi.
+      move=> /andP. move=> [LEa LEg] 
+                           [[A1 [B1 [R1 h1]]] [[A2 [B2 [R2 h2]]] h3]]. 
+
+      have [EQ1 EQ2]: A1 = A2 /\ B1 = B2. eapply HeadRed_tpi_det; eauto.
+      subst A2. subst B2.
+      move: h3 => [A3 [B3 [R3 h3]]].
+      have [EQ1 EQ2]: A1 = A3 /\ B1 = B3. eapply HeadRed_tpi_det; eauto.
+      subst A3. subst B3.
+
+      move: (andb_prop _ _ i0) => [Va Vg]. 
+      fold valid in Va.
+      fold valid in Vg. fold (valid_fun g) in Vg.
+      move: (andb_prop _ _ i2) => [Va0 Vg0]. 
+      fold valid in Va0. 
+      fold valid in Vg0. fold (valid_fun g0) in Vg0.
+      repeat split. 
+      ++ exists A1, B1. split; auto.
+         move=> u v INf P t0 APP0 TA VP.
+         have Vu : valid u. eauto with valid.
+         destruct (valid_app_exists Vg Vu) as [t [APP Vt]].
+         move: (le_fun_mono Vg Vg0 LEg Vu APP APP0) => LEt.
+         cbn.
+         eapply upVal. eapply LEt. eapply h1. eapply TA.
+         cbn.
+         eapply downVal. eapply LEa. eapply VP.
+         Unshelve. eapply INf. eapply APP.
+
+      ++ exists A1, B1. split; auto.
+         move=> u v INf P t0 APP0 TA VP.
+         have Vu : valid u. eauto with valid.
+         destruct (valid_app_exists Vg Vu) as [t [APP Vt]].
+         move: (le_fun_mono Vg Vg0 LEg Vu APP APP0) => LEt.
+         cbn.
+         eapply upVal. eapply LEt. eapply h2.  eapply TA.
+         cbn.
+         eapply downVal. eapply LEa. eapply VP.
+         Unshelve. eapply INf. eapply APP.
+
+      ++ exists A1, B1. split; auto.
+         move=> u v INf P t0 APP0 TA VP.
+         have Vu : valid u. eauto with valid.
+         destruct (valid_app_exists Vg Vu) as [t [APP Vt]].
+         move: (le_fun_mono Vg Vg0 LEg Vu APP APP0) => LEt.
+         eapply upEqVal. eapply LEt. eapply h3.  eapply TA.
+         eapply downVal. eapply LEa. eapply VP.
+         Unshelve. eapply INf. eapply APP.
+
+  - (* downVal *)
+    dependent destruction h1;
+    dependent destruction h0.
     all: try solve [cbn; eauto].
     + (* bot *)
       destruct a; destruct a0; cbn; auto; done.
     + (* tnat *)
-      all: move=> _ [RT [M1 [RM1 VM1]]].
-      split. auto. exists M1. split. auto.
+      all: move=> _ [M1 [RM1 VM1]].
+       exists M1. split. auto.
       eapply downVal with (a1 := tnat); eauto. 
     + (* tuniv *)
-      admit.
-    + move=> LE VM.
-      rewrite le_tpi in LE. move: LE => /andP. move=> [LEa LEg].
-      cbn in VM. cbn.
-      unfold ValPi in *.
-      move: VM => [A [B [RT PAV]]].
-      exists A, B. split. auto.
-      unfold PiAppVal in *.
-      move=> u v IN P t APP TP VP.
-      specialize (PAV u v IN P). 
-      have Vg : valid_fun  g. admit.
-      have Vg0 : valid_fun g0. admit.
-      have Vu : valid u. admit.
+      move=> LE VT.
+      cbn in LE. 
+      apply Nat.eqb_eq in LE. subst j0.
+      have EQ: (wt_tpi w w0 h0 i = wt_tpi w1 w2 h1 i0) by ext.
+      rewrite EQ.
+      eapply VT.
+    + (* tpi *)
+      rewrite le_tpi. cbn. unfold ValPi, PiAppVal.
+      move=> /andP. move=> [LEa LEg] [A [B [R1 h1]]]. 
+
+      move: (andb_prop _ _ i0) => [Va Vg]. 
+      fold valid in Va.
+      fold valid in Vg. fold (valid_fun g) in Vg.
+      move: (andb_prop _ _ i2) => [Va0 Vg0]. 
+      fold valid in Va0. 
+      fold valid in Vg0. fold (valid_fun g0) in Vg0.
+
+      exists A, B. split; auto.
+      move=> u v INf P t APP TA VP.
+      specialize (h1 u v INf P).
+      have Vu : valid u. eauto with valid.
       destruct (valid_app_exists Vg0 Vu) as [t0 [APP0 Vt0]].
       move: (le_fun_mono Vg Vg0 LEg Vu APP APP0) => LEt.
-      move: (wt_abs_key (wt_abs w1 w2 i i2) IN APP0) => h2.
-      remember (wt_abs_elt (wt_abs w1 w2 i i2) IN APP0) as h3.
-      eapply downVal with (a1 := t0)(h1:=h3). auto.
-      rewrite Heqh3.
-      eapply PAV; eauto.
+      eapply downVal. eapply LEt. eapply h1. eapply TA.
+      eapply upVal. eapply LEa. eapply VP.
+      Unshelve. eapply APP0.
+  - (* downEqVal *)
+    dependent destruction h1;
+    dependent destruction h0.
+    all: try solve [cbn; eauto].
+    + destruct a; destruct a0; cbn; auto; done.
+    + move=> _ [M1 [RM1 [N1 [RN1 VM1]]]].
+      exists M1. split. auto.
+      exists N1. split. auto.
+      eapply downEqVal with (a1 := tnat); eauto.
+    + (* tuniv *)
+      move=> LE VT.
+      cbn in LE. 
+      apply Nat.eqb_eq in LE. subst j0.
+      have EQ: (wt_tpi w w0 h0 i = wt_tpi w1 w2 h1 i0) by ext.
+      (* proof irrelevance for wt? this case doesn't use recursion *)
+      rewrite EQ.
+      eapply VT.
+    + (* tpi *)
+      rewrite le_tpi. cbn. unfold ValPi.
+      move=> /andP. move=> [LEa LEg] 
+                           [[A1 [B1 [R1 h1]]] [[A2 [B2 [R2 h2]]] h3]]. 
+
+      have [EQ1 EQ2]: A1 = A2 /\ B1 = B2. eapply HeadRed_tpi_det; eauto.
+      subst A2. subst B2.
+      move: h3 => [A3 [B3 [R3 h3]]].
+      have [EQ1 EQ2]: A1 = A3 /\ B1 = B3. eapply HeadRed_tpi_det; eauto.
+      subst A3. subst B3.
+
+      move: (andb_prop _ _ i0) => [Va Vg]. 
+      fold valid in Va.
+      fold valid in Vg. fold (valid_fun g) in Vg.
+      move: (andb_prop _ _ i2) => [Va0 Vg0]. 
+      fold valid in Va0. 
+      fold valid in Vg0. fold (valid_fun g0) in Vg0.
+      repeat split. 
+      ++ exists A1, B1. split; auto.
+         move=> u v INf P t APP TA VP.
+         have Vu : valid u. eauto with valid.
+         destruct (valid_app_exists Vg0 Vu) as [t0 [APP0 Vt0]].
+         move: (le_fun_mono Vg Vg0 LEg Vu APP APP0) => LEt.
+         eapply downVal. eapply LEt. eapply h1. eapply TA.
+         eapply upVal. eapply LEa. eapply VP.
+         Unshelve. eapply INf. eapply APP0.
+
+      ++ exists A1, B1. split; auto.
+         move=> u v INf P t APP TA VP.
+         have Vu : valid u. eauto with valid.
+         destruct (valid_app_exists Vg0 Vu) as [t0 [APP0 Vt0]].
+         move: (le_fun_mono Vg Vg0 LEg Vu APP APP0) => LEt.
+         eapply downVal. eapply LEt. eapply h2.  eapply TA.
+         eapply upVal. eapply LEa. eapply VP.
+         Unshelve. eapply INf. eapply APP0.
+      ++ exists A1, B1. split; auto.
+         move=> u v INf P t APP TA VP.
+         have Vu : valid u. eauto with valid.
+         destruct (valid_app_exists Vg0 Vu) as [t0 [APP0 Vt0]].
+         move: (le_fun_mono Vg Vg0 LEg Vu APP APP0) => LEt.
+         eapply downEqVal. eapply LEt. eapply h3.  eapply TA.
+         eapply upVal. eapply LEa. eapply VP.
+         Unshelve. eapply INf. eapply APP0.
 Admitted.
       
+
+
+(* ---- restrictVal / restrictEqVal: shrink the term-side u ---- *)
+
+(* restrictVal: same a, smaller u' ≤ u *)
+Fixpoint restrictVal M T u u' a
+  (h0 : wt u' a) (h1 : wt u a) {struct h1} :
+  le u' u -> Val M T h1 -> Val M T h0
+with restrictEqVal M N T u u' a 
+  (h0 : wt u' a) (h1 : wt u a) {struct h1} :
+  le u' u -> EqVal M N T h1 -> EqVal M N T h0.
+Proof. 
+  - dependent destruction h1. 
+    1 : { move=> h. apply le_bot_inv in h. subst.
+          have EQ: h0 = wt_bot i. ext. subst. auto. } 
+    all: dependent destruction h0.
+    all: try solve [cbn; eauto; try done].
+    + rewrite le_succ. cbn.
+      move=> LE [M1 [R1 V1]].
+      exists M1. split; auto.
+      eapply restrictVal; eauto.
+    + rewrite le_tpi. cbn.
+      move=> /andP. move=> [LEa LEf] [A [B [R1 [TA [TB [Vpi hT]]]]]].
+      move: hT => [Va [PEV PEEV]].
+      move: Vpi => /andP. fold (valid_fun g0).
+      move=> [Va0 Vg0].
+      exists A. exists B. repeat split; eauto.
+      ++ move=> u v INg N TN VN. cbn in *.
+         unfold PiEdgeVal in PEV.
+ Admitted.
+
+
+(* ---- down on ValTy / EqValTy ---- *)
+
+(* downValTy2 *)
+Lemma downValTy M u0 u1 i
+  (h0 : wt u0 (tuniv i)) (h1 : wt u1 (tuniv i)) :
+  le u0 u1 -> ValTy M h1 -> ValTy M h0.
+Proof. 
+    move=> LE VT1.
+    eapply Val_ValTy.
+    apply ValTy_Val in VT1.
+    eapply restrictVal; eauto.
+Qed.
+
+(* downEqValTy2 *)
+Lemma downEqValTy M N u0 u1 i
+  (h0 : wt u0 (tuniv i)) (h1 : wt u1 (tuniv i)) :
+  le u0 u1 -> EqValTy M N h1 -> EqValTy M N h0.
+Proof.
+    move=> LE VT1.
+    eapply EqVal_EqValTy.
+    apply EqValTy_EqVal in VT1.
+    eapply restrictEqVal; eauto.
+Qed.
+
+
+(* ---- Sup / lub ---- *)
+
+(* ValTy2-Sup: if a1 and a2 are universe-members and lub a1 a2 = Some a,
+   ValTy at a1 and a2 lifts to ValTy at the lub. *)
+Fixpoint ValTy_Sup T a1 a2 a i
+  (h1 : wt a1 (tuniv i)) (h2 : wt a2 (tuniv i)) (h : wt a (tuniv i)) {struct h}:
+  lub a1 a2 = Some a ->
+  ValTy T h1 -> ValTy T h2 -> ValTy T h.
+Proof. 
+  move=> LUB V1 V2.
+  unfold ValTy in *.
+  destruct a; try done.
+  destruct a1; destruct a2; inversion LUB; subst.
+  - have EQ: (h2 = h). ext. subst. done.
+  - destruct (n =? n0); try done.
+  - destruct (lub a1 a2) eqn:LUBa; inversion H0.
+  - have EQ: (h1 = h). ext. subst. done.
+  - destruct (compatible_fun l0 l1) eqn:CPT.
+    destruct (lub a1 a2) eqn:LUBa.
+    all: inversion H0.
+    subst.
+    inversion h. subst. 
+    move: V1 => [A1 [B1 [R1 [TA1 [TB1 [VT1 hV1]]]]]].
+    move: V2 => [A2 [B2 [R2 [TA2 [TB2 [VT2 hV2]]]]]].
+    have [EQ1 EQ2]: (A1 = A2) /\ B1 = B2.
+    eapply HeadRed_tpi_det; eauto. subst.
+    exists A2. exists B2.
+    repeat split; eauto.
+    move: hV1 => [VA1 [PE1 PEE1]].
+    move: hV2 => [VA2 [PE2 PEE2]].
+Admitted.    
+
+(* EqValTy2-Sup *)
+Lemma EqValTy_Sup M N a1 a2 a i
+  (h1 : wt a1 (tuniv i)) (h2 : wt a2 (tuniv i)) (h : wt a (tuniv i)) :
+  lub a1 a2 = Some a ->
+  EqValTy M N h1 -> EqValTy M N h2 -> EqValTy M N h.
+Proof. Admitted.
+
+
+(* ----------------------------------------------------- *)
 
 Fixpoint Val_EqVal_fwd M A u a (h : wt u a) B i (h' : wt a (tuniv i))
   {struct h} :
   Val M A h -> EqValTy A B h' -> Val M B h
 with EqVal_EqVal_fwd M N A u a (h : wt u a) B i (h' : wt a (tuniv i))
   {struct h} :
-  EqVal M N A h -> EqValTy A B h' -> EqVal M N B h.  
+  EqVal M N A h -> EqValTy A B h' -> EqVal M N B h
+with EqVal_sym M1 M2 A u a (h : wt u a) { struct h } : 
+  EqVal M1 M2 A h -> EqVal M2 M1 A h
+with EqVal_trans M1 M2 M3 A u a (h : wt u a) {struct h} :
+  EqVal M1 M2 A h -> EqVal M2 M3 A h -> EqVal M1 M3 A h.
 Proof.
-(*
-  have EqValPi_EqVal_fwd : forall
-      M A f a g (h : wt (abs f) (tpi a g)) B i (h' : wt a (tuniv i)),
-   ValPi M A h -> EqValTy A B h' -> ValPi M B h.
-  { 
-    clear M A u a h B i h'.
-    move=> M A f a g h B i h'.
-    unfold ValPi.
-    move=> [A0 [B0 [R0 PAV0]]] h1.
-    admit.
-  } *)
-  - dependent destruction h.
+  - (* Val_EqVal_fwd *)
+    dependent destruction h.
     all: dependent destruction h'.
     all: cbn.
     all: eauto.    
-    + (* tnat *)
-      admit. (* !!!!! *)
-    + (* zero *) 
-      admit.
-    + (* succ *)
-      admit.
-    + (* abs *)
-      unfold ValPi.
-      move=> [A0 [B0 [RA PAV]]].
+    + move=> [A' [B' [RA' PAV]]].
       move=> [hA [hB hAB]].
-      destruct hB as (A1 & B1 & RB & hB).
-      exists A1, B1. split. exact RB.
-      unfold PiAppVal.
-      move=> u v IN P t APP tP VPA1.
-Admitted.      
-
-Fixpoint EqVal_sym M N A u a (h : wt u a) {struct h} : 
-  EqVal M N A h -> EqVal N M A h.
-Proof.
-  dependent destruction h.
-  all: cbn.
-  all: eauto.
-  (* 4 nontrivial *)
-  - destruct a; try done.
-  - move=> [h1 [M1 [h2 [N1 [h3 E]]]]].
-    repeat split; eauto.
-    exists N1. eauto.
-  - move=> [vpiM [vPiN [_ [_ h3]]]].
-    repeat split; eauto.
-    clear A.
-    move: h3 => [A0 [B0 [R1 [A1 [B1 [R2 [T1 [T2 [Vt [EA PEE]]]]]]]]]].
-    eexists. eexists.
-    repeat split; eauto.
-    eexists. eexists.
-    repeat split; eauto.
-    eapply c_sym; eauto.
-    eapply c_sym; eauto.
-    eapply ctx_conv_conv; eauto.
-    move=> u v IN P TA1 VP.
-    have TA0: typing ctx_empty P A0.
-    { eauto using t_conv, c_sym. }
-    specialize (PEE u v IN P TA0).
-    eapply EqVal_EqValTy.
-    eapply EqVal_sym; eauto.
-    eapply EqValTy_EqVal; eauto.
-    eapply PEE; eauto.
-Admitted.
-
-(* Fundamental theorem for the logical relation 
-   
-   We want to show that well-typed terms are in the 
-   relation.
-
-   - If Γ |- M : A (typing) then
-
-
-     if Γ |= ρ ~ σ  (ValSub)
-
-          and  Γ |- σ  (typing_subst ctx_empty)
-
-          and  Γ |= ρ  (fits)   
-
-
-     for all u, a, such that h ∈ u : a   (wt)
-
-        where [[M]]ρ = u  and [[A]]ρ = a  (EvalRel)
-
-     we have
-
-        Val u a M[σ] A[σ] h
-
-   - If Γ |- M = N : A  (conv) 
-
-     and  Γ |- σ1  Γ |- σ2 (typing_subst ctx_empty)
-
-     and  Γ |= ρ  (fits)   
-
-     and [[M]]ρ = u and [[N]]ρ = u and [[A]]ρ = a  (EvalRel)
- 
-     and h ∈ u : a   (wt)
-
-     and Γ |= ρ ~ σ1 == σ2   (EqValSub)
-
-     then
-
-     EqVal u a M[σ1] N[σ2] A[σ] h
-*)
-
-
-(* A closing substitution: σ *)
-Definition Sub m := fin m -> Tm O.
-
-(* A valid closing substitution σ maps every term to one that 
-   can be interpreted. *) 
-Definition ValSub {g} (Γ : Ctx g) (ρ : Env g) (σ : Sub g)  : Prop := 
-  forall i,
-  forall u, valid u -> le u (ρ i) ->
-    forall a, EvalRel (lookup i Γ) ρ a ->
-    forall (h : wt u a), 
-      Val (σ i) (lookup i Γ)[σ] h. 
-
-
-Lemma ValSub_empty : ValSub ctx_empty null null.
-unfold ValSub. done. Qed.
-
-Lemma ValSub_cons {g} (Γ : Ctx g) (ρ : Env g) (σ : Sub g) A v (M : Tm 0): 
-    (forall u, valid u -> le u v -> forall a (h : wt u a),
-    EvalRel A ρ a -> 
-    Val M A[σ] h) -> 
-    ValSub Γ ρ σ -> 
-    ValSub (Γ ++ A) (v .: ρ) (M .: σ). 
-Proof.
-  intros hyp0 VS.
-  unfold ValSub in *.
-  move=> i u0 Vu0 Le0 a0 E0 WT0.
-  destruct i as [i|].
-  - (* succ case *) 
-    cbn in *. asimpl.
+      destruct hA as (A0 & B0 & RA0 & hA).
+      destruct hB as (A1 & B1 & RB1 & hB).
+      have [EQ1 EQ2]: A' = A0 /\ B' = B0.
+      eapply HeadRed_tpi_det; eauto. subst A'. subst B'. clear RA'.
+      exists A1, B1. split. exact RB1.
+      unfold PiAppVal. cbn.
+      move=> u v IN P t APP tP VPA1. 
+      unfold PiAppVal in PAV.
+      specialize (PAV u v IN P t APP).
+      admit.
+  - (* EqVal_EqVal_fwd *)
     admit.
-  - (* zero case *)
-    cbn in *. asimpl.
-    eapply EvalRel_unwk in E0; auto.
+  - (* EqVal_sym *)
+    dependent destruction h.
+    all: cbn.
+    all: eauto.
+    (* 4 nontrivial *)
+    + destruct a; try done.
+    + move=> [M3 [RM3 [N3 [RN2 EV3]]]].
+      have EQ: (M3 = N3). admit. (* HeadRed_succ_det *)
+      subst.
+      exists N3. split; auto.
+      exists N3. split; auto.
+    + move=> [vpiM [vPiN [_ [_ h3]]]].
+      repeat split; eauto.
+      clear A.
+      move: h3 => [A0 [B0 [R1 [A1 [B1 [R2 [T1 [T2 [Vt [EA PEE]]]]]]]]]].
+      eexists. eexists.
+      repeat split; eauto.
+      eexists. eexists.
+      repeat split; eauto.
+      eapply c_sym; eauto.
+      eapply c_sym; eauto.
+      eapply ctx_conv_conv; eauto.
+      move=> u v IN P TA1 VP.
+      have TA0: typing ctx_empty P A0.
+      { eauto using t_conv, c_sym. }
+      specialize (PEE u v IN P TA0).
+      eapply EqVal_EqValTy.
+      eapply EqVal_sym; eauto.
+      eapply EqValTy_EqVal; eauto.
+      eapply PEE; eauto.
+      eapply Val_EqVal_fwd. eapply VP.
+      eapply EqVal_EqValTy. 
+      eapply EqVal_sym; eauto.
+    + move=> [VP1 [VP2 EP1]].
+      repeat split; auto.
+      unfold EqValPi in *.
+      move: EP1 => [A1 [A2 [R1 PAV]]].
+      exists A1. exists A2. 
+      repeat split; auto.
+      unfold PiAppEqVal in *.
+      move=> u v IN P t APP TPA VP.
+      specialize (PAV u v IN P t APP TPA VP).
+      cbn in PAV. cbn.
+      eapply EqVal_sym; eauto.
+  - (* EqVal_trans *)
 Admitted.
 
-Definition EqValSub {g} (Γ : Ctx g) (ρ : Env g) 
-  (σ1 : Sub g) (σ2 : Sub g)  : Prop := 
-  forall i, 
-  forall u, valid u -> le u (ρ i) ->
-    forall a, EvalRel (lookup i Γ) ρ a ->
-    forall (h : wt u a), 
-      EqVal (σ1 i) (σ2 i) (lookup i Γ)[σ1] h. 
 
-Lemma EqValSub_empty : EqValSub ctx_empty null null null.
-unfold EqValSub. done. Qed.
 
-Lemma EqValSub_cons {g} (Γ : Ctx g) (ρ : Env g) 
-  (σ1 σ2 : Sub g) A v (M1 M2 : Tm 0): 
-    (forall u, valid u -> le u v -> forall a (h : wt u a),
-    EvalRel A ρ a -> 
-    EqVal M1 M2 A[σ1] h) -> 
-    EqValSub Γ ρ σ1 σ2 -> 
-    EqValSub (Γ ++ A) (v .: ρ) (M1 .: σ1) (M2 .: σ2). 
-Proof.
-  intros hyp0 VS.
-  unfold ValSub in *.
-  move=> i u0 Vu0 Le0 a0 E0 WT0.
-  destruct i as [i|].
-  - (* succ case *) 
-    cbn in *. asimpl.
-    admit.
-  - (* zero case *)
-    cbn in *. asimpl.
-    eapply EvalRel_unwk in E0; auto.
-Admitted.
-
-Definition semantic_typing {n} (Γ : Ctx n) (M : Tm n) (A : Tm n) :=
-  forall ρ σ (TS : typing_subst ctx_empty σ Γ) (F : fits Γ ρ) 
-    (VS : ValSub Γ ρ σ), 
-  forall u a (WT : wt u a), 
-    EvalRel M ρ u -> 
-    EvalRel A ρ a -> 
-    Val M[σ] A[σ] WT.
-Definition semantic_conv {n} (Γ : Ctx n) (M N: Tm n) (A : Tm n) :=
-  forall ρ σ (TS : typing_subst ctx_empty σ Γ) (F : fits Γ ρ)
-    (VS : ValSub Γ ρ σ), 
-  forall u a (WT : wt u a), 
-    EvalRel M ρ u -> 
-    EvalRel A ρ a -> 
-    EqVal M[σ] N[σ] A[σ] WT. 
-Definition semantic_conv2 {n} (Γ : Ctx n) (M N: Tm n) (A : Tm n) :=
-  forall ρ σ1 σ2 (TS1 : typing_subst ctx_empty σ1 Γ) 
-            (TS2 : typing_subst ctx_empty σ2 Γ)
-    (F : fits Γ ρ)
-    (VS : EqValSub Γ ρ σ1 σ2), 
-  forall u a (WT : wt u a), 
-    EvalRel M ρ u -> 
-    EvalRel A ρ a -> 
-    EqVal M[σ1] N[σ2] A[σ1] WT. 
-
-Notation "Γ ⊨ M ∈ A" := (semantic_typing Γ M A) (at level 70).
-Notation "Γ ⊨ M ≡ N ∈ A" := (semantic_conv2 Γ M N A) (at level 70).
-
-(* ------------------ semantic typing rules ----------- *)
-
-Section SemanticTyping.
-
-Variable (n:nat) (Γ : Ctx n).
-
-Lemma st_var (x : fin n) : 
-  ctx Γ -> 
-(* ------------------------- *)
-  Γ ⊨ var x ∈ lookup x Γ.
-Proof.
-  move=> h. 
-  move=> ρ σ TS FR VS u1 a1 WT1 Ex ER.
-  cbn in *. move: Ex => [Vu1 Le1].
-  specialize (VS x).
-  eapply VS; eauto.
+(* EqValTy2-sym *)
+Lemma EqValTy_sym M N u i (h : wt u (tuniv i)) :
+  EqValTy M N h -> EqValTy N M h.
+Proof. 
+  move=>h1. eapply EqVal_EqValTy. eapply EqVal_sym.
+  eapply EqValTy_EqVal. done.
 Qed.
 
-Lemma st_conv M A B i : 
-  Γ ⊨ M ∈ A -> 
-  Γ ⊨ A ≡ B ∈ Core.tuniv i ->
-(* ------------------------- *)
-  Γ ⊨ M ∈ B.
-Proof.
-  move=> h1 h2. 
-  move=> ρ σ TS FR VS u1 a1 WT1 Ex ER.
-  specialize (h1 ρ σ TS FR VS).
-  specialize (h2 ρ σ σ TS TS FR).
-Admitted.  
+(* EqValTy2-trans *)
+Lemma EqValTy_trans A B C u i (h : wt u (tuniv i)) :
+  EqValTy A B h -> EqValTy B C h -> EqValTy A C h.
+Proof. 
+  move=> h1 h2.
+  eapply EqVal_EqValTy. eapply EqVal_trans.
+  eapply EqValTy_EqVal. eauto.
+  eapply EqValTy_EqVal. eauto.
+Qed.
 
-Lemma st_abs A B M i : 
-  Γ ⊨ A ∈ Core.tuniv i -> 
-  Γ ++ A ⊨ B ∈ Core.tuniv i -> 
-  Γ ++ A ⊨ M ∈ B ->
-(* ------------------------- *)
-  Γ ⊨ Core.abs A M ∈ Core.tpi A B.
-Admitted.
+(* ============================================================
+   Translations of theorem statements from Validity2.agda
+   ------------------------------------------------------------
 
-Lemma st_app A B N M i : 
-(*  Γ |- A ∈ Core.tuniv i -> 
-  Γ ++ A |- B ∈ Core.tuniv i -> 
-  Γ |- M ∈ (Core.tpi A B) -> 
-  Γ |- N ∈ A  ->  *)
-  Γ ⊨ A ∈ Core.tuniv i -> 
-  Γ ++ A ⊨ B ∈ Core.tuniv i -> 
-  Γ ⊨ M ∈ (Core.tpi A B) -> 
-  Γ ⊨ N ∈ A  -> 
-(* ------------------------ *)
-  Γ ⊨ Core.app M N ∈ B[N..].
-Proof.
-  move=> h1 h2 h3 h4 (* h1' h2' h3' h4' *). 
-  move=> ρ σ TS FR VS u1 a1 WT1 Ex ER.
-  specialize (h1 ρ σ TS FR VS).
-  specialize (h3 ρ σ TS FR VS).
-  specialize (h4 ρ σ TS FR VS).
-  cbn.
-  cbn in Ex.
-  destruct (is_bot u1) eqn:HB. 
-  - (* EvalRel (app M N) is bot *)
-    destruct u1; try done.
-    dependent destruction WT1. cbn.
-    destruct a; try done.
-    admit.
-  - (* EvalRel (app M N) comes from an application *)
-    move: Ex => [u0 [EM EN]].    
-    move: (h3 (u0 ↦ u1)) => h3'.
-    (* we need to get a type for (u0 |-> u1). *)
-Admitted.
- 
+   Translation conventions (Agda → Rocq):
+     FinMem u a              ≈  wt u a
+     FinMem b UCode          ≈  wt b (tuniv i)         (some i)
+     Coherent u              ≈  valid u                (implicit in wt)
+     CoherentFun g           ≈  valid_fun g            (implicit in wt (abs g) ..)
+     CoherentFunTail f       ≈  valid_fun f            (implicit in wt (tpi _ f) ..)
+     FinMemFun g b f         ≈  wt (abs g) (tpi b f)
+     FinMemAllU f b          ≈  wt (tpi b f) (tuniv i) (codomains in U_i)
+     LeCode u v              ≈  le u v
+     LeFunCode f g           ≈  le_fun f g
+     Comp u v                ≈  compatible u v
+     Sup u v = w             ≈  lub u v = Some w
+     Selection f u v         ≈  In (u, v) f
+     EvalFun f u = v         ≈  app f u = Some v
+     subst1 B N              ≈  B[N..]
+     HasType / ConvTm        ≈  typing / conv
+     HeadRed                 ≈  HeadRed (multi reduction)
 
-End SemanticTyping.
+   Closed terms (Tm 0) are used throughout.
 
+   ------------------------------------------------------------
+   Dependency stratification of the mutual block.
 
- 
-(* 
-  -- Main bundled adequacy theorem
-  adequacySub2 : {h g : Nat} {H : Ctx h} {G : Ctx g}
-    {M A : Expr g} ->
-    HasType G M A ->       (* syntax.typing *)
-    (sigma : Sub h g) -> 
-    (rho : EnvApprox g) ->  (* Env *)
-    CoherentEnv rho ->  (* valid_env *)
-    ValidSub2 H G sigma rho -> 
-    Fits G rho ->
-    WtSub H G sigma -> WfCtx H ->
-    (u : FinEl) -> EvalRel M rho u ->
-    (a : FinEl) -> EvalRel A rho a -> FinMem u a ->
-    Val2 H (substExpr sigma M) (substExpr sigma A) u a
+   The Agda mutual block of Validity2.agda decomposes into the
+   following strongly-connected components, in topological order
+   (a level may only call itself or earlier levels):
 
-  -- Bundled adequacy for conversion
-  adequacyEqSub2 : {h g : Nat} {H : Ctx h} {G : Ctx g}
-    {M N A : Expr g} ->
-    ConvTm G M N A ->
-    (sigma : Sub h g) -> (rho : EnvApprox g) ->
-    CoherentEnv rho -> ValidSub2 H G sigma rho -> Fits G rho ->
-    WtSub H G sigma -> WfCtx H ->
-    (u : FinEl) -> EvalRel M rho u ->
-    (a : FinEl) -> EvalRel A rho a -> FinMem u a ->
-    EqVal2 H (substExpr sigma M) (substExpr sigma N) (substExpr sigma A) u a
+     Level 1 (no recursive calls in the mutual block):
+       - EqVal_Val1                   (Val2-from-EqVal2-first)
+       - EqVal_Val2                   (Val2-from-EqVal2-second)
+       - ValTy_headred_expand         (ValTy2-headred-expand)
+       - ValTy_headred_contract       (ValTy2-headred-contract)
 
-  -- Two-substitution adequacy
-  adequacyConvSub2 : {h g : Nat} {H : Ctx h} {G : Ctx g}
-    {M A : Expr g} ->
-    HasType G M A ->
-    (sigma sigma' : Sub h g) -> (rho : EnvApprox g) ->
-    CoherentEnv rho ->
-    ValidSub2 H G sigma rho -> ValidSub2 H G sigma' rho ->
-    ValidConvSub2 H G sigma sigma' rho ->
-    Fits G rho ->
-    WtSub H G sigma -> WtSub H G sigma' ->
-    WtConvSub H G sigma sigma' ->
-    WfCtx H ->
-    (u : FinEl) -> EvalRel M rho u ->
-    (a : FinEl) -> EvalRel A rho a -> FinMem u a ->
-    EqVal2 H (substExpr sigma M) (substExpr sigma' M) (substExpr sigma A) u a
+     Level 2 (calls into Level 1 only):
+       - EqValTy_headred_expand       (uses ValTy_headred_expand)
+       - EqValTy_headred_contract     (uses ValTy_headred_contract)
 
-*)
+     Level 3 (4-way SCC, plus dependencies on Levels 1-2):
+       Val_beta_expand  ↔  ValPi_headred_expand
+                        ↔  EqVal_headred_expand
+                        ↔  EqValPi_headred_expand
+
+     Level 4 (4-way SCC, plus dependencies on Levels 1-2):
+       Val_headred_contract  ↔  ValPi_headred_contract
+                             ↔  EqVal_headred_contract
+                             ↔  EqValPi_headred_contract
+
+     Level 5 (2-way SCC, independent of Levels 3-4):
+       Val_EqVal  ↔  ValTy_EqValTy
+
+     Level 6 (BIG SCC, ~30 lemmas, depends only on Levels 1, 5):
+       { EqValTy_sym, EqValTy_trans, EqVal_sym, EqVal_trans,
+         Val_EqVal_fwd, EqVal_EqVal_fwd, ValTy_Sup, EqValTy_Sup,
+         downVal, downEqVal, downValTy, downEqValTy,
+         upVal, upEqVal, restrictVal, restrictEqVal,
+         downPiAppVal, downPiAppEq, downPiAppEqVal,
+         upPiAppVal, upPiAppEq, upPiAppEqVal,
+         transportPiEdgeVal_sel, transportPiEdgeEq_sel,
+         transportPiEdgeEqTy_sel,
+         restrictPiAppVal_sel, restrictPiAppEq_sel,
+         restrictPiAppEqVal_sel,
+         restrictVal_PiCode, restrictEqVal_PiCode }
+
+     Cycles in Level 6 (sample):
+       downVal → downValTy → transportPiEdgeVal_sel → upVal
+              → upPiAppVal → downVal
+       restrictVal → restrictVal_PiCode → restrictPiAppVal_sel
+                   → restrictVal
+       Val_EqVal_fwd → restrictVal → upPiAppVal → ... → Val_EqVal_fwd
+   ============================================================ *)
 
 
 
-  
+(* ============================================================
+   Level 2 — depends on Level 1
+   ============================================================ *)
+
+(* EqValTy2-headred-expand *)
+Lemma EqValTy_headred_expand M1 M2 M1' M2' u i (h : wt u (tuniv i)) :
+  HeadRed M1' M1 -> HeadRed M2' M2 ->
+  EqValTy M1 M2 h -> EqValTy M1' M2' h.
+Proof. Admitted.
+
+(* EqValTy2-headred-contract *)
+Lemma EqValTy_headred_contract M1 M2 M1' M2' u i (h : wt u (tuniv i)) :
+  HeadRed M1 M1' -> HeadRed M2 M2' ->
+  EqValTy M1 M2 h -> EqValTy M1' M2' h.
+Proof. Admitted.
+
+
+(* ============================================================
+   Level 3 — 4-way SCC for HeadRed expand on Val/EqVal/ValPi/EqValPi
+   ============================================================ *)
+
+(* Val2-beta-expand *)
+Lemma Val_beta_expand M M' T u a (h : wt u a) :
+  HeadRed M' M -> Val M T h -> Val M' T h.
+Proof. Admitted.
+
+(* EqVal2-headred-expand *)
+Lemma EqVal_headred_expand M M' N N' T u a (h : wt u a) :
+  HeadRed M' M -> HeadRed N' N ->
+  EqVal M N T h -> EqVal M' N' T h.
+Proof. Admitted.
+
+(* ValPi2-headred-expand *)
+Lemma ValPi_headred_expand M M' T b f g (h : wt (abs g) (tpi b f)) :
+  HeadRed M' M -> ValPi M T h -> ValPi M' T h.
+Proof. Admitted.
+
+(* EqValPi2-headred-expand *)
+Lemma EqValPi_headred_expand M1 M2 M1' M2' T b f g
+  (h : wt (abs g) (tpi b f)) :
+  HeadRed M1' M1 -> HeadRed M2' M2 ->
+  EqValPi M1 M2 T h -> EqValPi M1' M2' T h.
+Proof. Admitted.
+
+
+(* ============================================================
+   Level 4 — 4-way SCC for HeadRed contract
+   ============================================================ *)
+
+(* Val2-headred-contract *)
+Lemma Val_headred_contract M M' T u a (h : wt u a) :
+  HeadRed M M' -> Val M T h -> Val M' T h.
+Proof. Admitted.
+
+(* EqVal2-headred-contract *)
+Lemma EqVal_headred_contract M M' N N' T u a (h : wt u a) :
+  HeadRed M M' -> HeadRed N N' ->
+  EqVal M N T h -> EqVal M' N' T h.
+Proof. Admitted.
+
+(* ValPi2-headred-contract *)
+Lemma ValPi_headred_contract M M' T b f g (h : wt (abs g) (tpi b f)) :
+  HeadRed M M' -> ValPi M T h -> ValPi M' T h.
+Proof. Admitted.
+
+(* EqValPi2-headred-contract *)
+Lemma EqValPi_headred_contract M1 M2 M1' M2' T b f g
+  (h : wt (abs g) (tpi b f)) :
+  HeadRed M1 M1' -> HeadRed M2 M2' ->
+  EqValPi M1 M2 T h -> EqValPi M1' M2' T h.
+Proof. Admitted.
+
+
+
+
+(* ============================================================
+   Level 6 (BIG SCC) — symmetry, transitivity, fwd-along-EqValTy,
+   sup, up/down, restrict, and all Pi helper lemmas.
+   ============================================================ *)
+
+(* ---- Symmetry / transitivity ---- *)
+
+
+
+
+
+
+
+(* ---- Pi helper lemmas: down/up/transport/restrict on PiApp / PiEdge ---- *)
+
+(* downPiAppVal2: PiAppVal at (b1, f1) transports down to (b0, f0)
+   when b0 ≤ b1 and f0 ≤ f1, given that A0 is a type at b1. *)
+Lemma downPiAppVal M A0 (B0 : Tm 1) b0 f0 b1 f1 g i
+  (h0 : wt (abs g) (tpi b0 f0))
+  (h1 : wt (abs g) (tpi b1 f1))
+  (hPi0 : wt (tpi b0 f0) (tuniv i))
+  (hPi1 : wt (tpi b1 f1) (tuniv i))
+  (hb1 : wt b1 (tuniv i)) :
+  le b0 b1 -> le_fun f0 f1 ->
+  ValTy A0 hb1 ->
+  PiAppVal M A0 B0 h1 -> PiAppVal M A0 B0 h0.
+Proof. Admitted.
+
+(* downPiAppEq2 *)
+Lemma downPiAppEq M A0 (B0 : Tm 1) b0 f0 b1 f1 g i
+  (h0 : wt (abs g) (tpi b0 f0))
+  (h1 : wt (abs g) (tpi b1 f1))
+  (hPi0 : wt (tpi b0 f0) (tuniv i))
+  (hPi1 : wt (tpi b1 f1) (tuniv i))
+  (hb1 : wt b1 (tuniv i)) :
+  le b0 b1 -> le_fun f0 f1 ->
+  ValTy A0 hb1 ->
+  (* Agda PiAppEq2 (no Rocq notation yet); paraphrase: *)
+  (forall u v (IN : In (u,v) g) (N1 N2 : Tm 0) t (APP : app f1 u = Some t),
+      typing ctx_empty N1 A0 -> typing ctx_empty N2 A0 ->
+      conv ctx_empty N1 N2 A0 ->
+      EqVal N1 N2 A0 (wt_abs_key h1 IN APP) ->
+      EqVal (Core.app M N1) (Core.app M N2) B0[N1..]
+            (wt_abs_elt h1 IN APP)) ->
+  (forall u v (IN : In (u,v) g) (N1 N2 : Tm 0) t (APP : app f0 u = Some t),
+      typing ctx_empty N1 A0 -> typing ctx_empty N2 A0 ->
+      conv ctx_empty N1 N2 A0 ->
+      EqVal N1 N2 A0 (wt_abs_key h0 IN APP) ->
+      EqVal (Core.app M N1) (Core.app M N2) B0[N1..]
+            (wt_abs_elt h0 IN APP)).
+Proof. Admitted.
+
+(* downPiAppEqVal2 *)
+Lemma downPiAppEqVal M N A0 (B0 : Tm 1) b0 f0 b1 f1 g i
+  (h0 : wt (abs g) (tpi b0 f0))
+  (h1 : wt (abs g) (tpi b1 f1))
+  (hPi0 : wt (tpi b0 f0) (tuniv i))
+  (hPi1 : wt (tpi b1 f1) (tuniv i))
+  (hb1 : wt b1 (tuniv i)) :
+  le b0 b1 -> le_fun f0 f1 ->
+  ValTy A0 hb1 ->
+  PiAppEqVal M N A0 B0 h1 -> PiAppEqVal M N A0 B0 h0.
+Proof. Admitted.
+
+(* upPiAppVal2 *)
+Lemma upPiAppVal M A0 (B0 : Tm 1) b0 f0 b1 f1 g i
+  (h0 : wt (abs g) (tpi b0 f0))
+  (h1 : wt (abs g) (tpi b1 f1))
+  (hPi0 : wt (tpi b0 f0) (tuniv i))
+  (hPi1 : wt (tpi b1 f1) (tuniv i)) :
+  le b0 b1 -> le_fun f0 f1 ->
+  PiEdgeVal A0 B0 hPi1 ->
+  PiAppVal M A0 B0 h0 -> PiAppVal M A0 B0 h1.
+Proof. Admitted.
+
+(* upPiAppEq2 *)
+Lemma upPiAppEq M A0 (B0 : Tm 1) b0 f0 b1 f1 g i
+  (h0 : wt (abs g) (tpi b0 f0))
+  (h1 : wt (abs g) (tpi b1 f1))
+  (hPi0 : wt (tpi b0 f0) (tuniv i))
+  (hPi1 : wt (tpi b1 f1) (tuniv i)) :
+  le b0 b1 -> le_fun f0 f1 ->
+  PiEdgeVal A0 B0 hPi1 ->
+  (forall u v (IN : In (u,v) g) (N1 N2 : Tm 0) t (APP : app f0 u = Some t),
+      typing ctx_empty N1 A0 -> typing ctx_empty N2 A0 ->
+      conv ctx_empty N1 N2 A0 ->
+      EqVal N1 N2 A0 (wt_abs_key h0 IN APP) ->
+      EqVal (Core.app M N1) (Core.app M N2) B0[N1..]
+            (wt_abs_elt h0 IN APP)) ->
+  (forall u v (IN : In (u,v) g) (N1 N2 : Tm 0) t (APP : app f1 u = Some t),
+      typing ctx_empty N1 A0 -> typing ctx_empty N2 A0 ->
+      conv ctx_empty N1 N2 A0 ->
+      EqVal N1 N2 A0 (wt_abs_key h1 IN APP) ->
+      EqVal (Core.app M N1) (Core.app M N2) B0[N1..]
+            (wt_abs_elt h1 IN APP)).
+Proof. Admitted.
+
+(* upPiAppEqVal2 *)
+Lemma upPiAppEqVal M N A0 (B0 : Tm 1) b0 f0 b1 f1 g i
+  (h0 : wt (abs g) (tpi b0 f0))
+  (h1 : wt (abs g) (tpi b1 f1))
+  (hPi0 : wt (tpi b0 f0) (tuniv i))
+  (hPi1 : wt (tpi b1 f1) (tuniv i)) :
+  le b0 b1 -> le_fun f0 f1 ->
+  PiEdgeVal A0 B0 hPi1 ->
+  PiAppEqVal M N A0 B0 h0 -> PiAppEqVal M N A0 B0 h1.
+Proof. Admitted.
+
+(* transportPiEdgeVal2-sel: PiEdgeVal at (b1, f1) transports to (b0, f0)
+   when b0 ≤ b1, f0 ≤ f1 and A is a type at b1. *)
+Lemma transportPiEdgeVal_sel A (B : Tm 1) b0 f0 b1 f1 i
+  (hPi0 : wt (tpi b0 f0) (tuniv i))
+  (hPi1 : wt (tpi b1 f1) (tuniv i))
+  (hb1  : wt b1 (tuniv i)) :
+  le b0 b1 -> le_fun f0 f1 ->
+  ValTy A hb1 ->
+  PiEdgeVal A B hPi1 -> PiEdgeVal A B hPi0.
+Proof. Admitted.
+
+(* transportPiEdgeEq2-sel *)
+Lemma transportPiEdgeEq_sel A (B : Tm 1) b0 f0 b1 f1 i
+  (hPi0 : wt (tpi b0 f0) (tuniv i))
+  (hPi1 : wt (tpi b1 f1) (tuniv i))
+  (hb1  : wt b1 (tuniv i)) :
+  le b0 b1 -> le_fun f0 f1 ->
+  ValTy A hb1 ->
+  PiEdgeEqVal A B hPi1 -> PiEdgeEqVal A B hPi0.
+Proof. Admitted.
+
+(* transportPiEdgeEqTy2-sel: PiEdgeEqTy at (b1, f1) transports to (b0, f0).
+   PiEdgeEqTy is the inlined "for all P : A. EqValTy B[P..] B'[P..]" piece
+   that appears inside Rec.EqValTy on the tpi case. *)
+Lemma transportPiEdgeEqTy_sel A (B B' : Tm 1) b0 f0 b1 f1 i
+  (hPi0 : wt (tpi b0 f0) (tuniv i))
+  (hPi1 : wt (tpi b1 f1) (tuniv i))
+  (hb1  : wt b1 (tuniv i)) :
+  le b0 b1 -> le_fun f0 f1 ->
+  ValTy A hb1 ->
+  (forall u v (IN : In (u,v) f1) (P : Tm 0),
+      typing ctx_empty P A ->
+      Val P A (wt_tpi_cod_key hPi1 IN) ->
+      EqValTy B[P..] B'[P..] (wt_tpi_cod_elt hPi1 IN)) ->
+  (forall u v (IN : In (u,v) f0) (P : Tm 0),
+      typing ctx_empty P A ->
+      Val P A (wt_tpi_cod_key hPi0 IN) ->
+      EqValTy B[P..] B'[P..] (wt_tpi_cod_elt hPi0 IN)).
+Proof. Admitted.
+
+(* restrictPiAppVal2-sel: restrict the function-domain g to a smaller g'. *)
+Lemma restrictPiAppVal_sel M A0 (B0 : Tm 1) b f g g' i
+  (h  : wt (abs g)  (tpi b f))
+  (h' : wt (abs g') (tpi b f))
+  (hPi : wt (tpi b f) (tuniv i)) :
+  le_fun g' g ->
+  PiEdgeVal A0 B0 hPi ->
+  PiAppVal M A0 B0 h -> PiAppVal M A0 B0 h'.
+Proof. Admitted.
+
+(* restrictPiAppEq2-sel *)
+Lemma restrictPiAppEq_sel M A0 (B0 : Tm 1) b f g g' i
+  (h  : wt (abs g)  (tpi b f))
+  (h' : wt (abs g') (tpi b f))
+  (hPi : wt (tpi b f) (tuniv i)) :
+  le_fun g' g ->
+  PiEdgeVal A0 B0 hPi ->
+  (forall u v (IN : In (u,v) g) (N1 N2 : Tm 0) t (APP : app f u = Some t),
+      typing ctx_empty N1 A0 -> typing ctx_empty N2 A0 ->
+      conv ctx_empty N1 N2 A0 ->
+      EqVal N1 N2 A0 (wt_abs_key h IN APP) ->
+      EqVal (Core.app M N1) (Core.app M N2) B0[N1..]
+            (wt_abs_elt h IN APP)) ->
+  (forall u v (IN : In (u,v) g') (N1 N2 : Tm 0) t (APP : app f u = Some t),
+      typing ctx_empty N1 A0 -> typing ctx_empty N2 A0 ->
+      conv ctx_empty N1 N2 A0 ->
+      EqVal N1 N2 A0 (wt_abs_key h' IN APP) ->
+      EqVal (Core.app M N1) (Core.app M N2) B0[N1..]
+            (wt_abs_elt h' IN APP)).
+Proof. Admitted.
+
+(* restrictPiAppEqVal2-sel *)
+Lemma restrictPiAppEqVal_sel M N A0 (B0 : Tm 1) b f g g' i
+  (h  : wt (abs g)  (tpi b f))
+  (h' : wt (abs g') (tpi b f))
+  (hPi : wt (tpi b f) (tuniv i)) :
+  le_fun g' g ->
+  PiEdgeVal A0 B0 hPi ->
+  PiAppEqVal M N A0 B0 h -> PiAppEqVal M N A0 B0 h'.
+Proof. Admitted.
+
+(* restrictVal2-PiCode *)
+Lemma restrictVal_PiCode M T b f g g' i
+  (h  : wt (abs g)  (tpi b f))
+  (h' : wt (abs g') (tpi b f))
+  (hPi : wt (tpi b f) (tuniv i)) :
+  le_fun g' g ->
+  ValTy T hPi ->
+  ValPi M T h -> ValPi M T h'.
+Proof. Admitted.
+
+(* restrictEqVal2-PiCode *)
+Lemma restrictEqVal_PiCode M N T b f g g' i
+  (h  : wt (abs g)  (tpi b f))
+  (h' : wt (abs g') (tpi b f))
+  (hPi : wt (tpi b f) (tuniv i)) :
+  le_fun g' g ->
+  ValTy T hPi ->
+  EqValPi M N T h -> EqValPi M N T h'.
+Proof. Admitted.
+
